\documentclass{article}
\usepackage{amsmath}

\begin{document}

% Image 1 content appears to be missing or blank

% Image 2 content
Let $G$ be a group. Let $H \triangleleft G$. Let $K = G/H$. Then:
\begin{align*}
\phi: G &\to K \\
g &\mapsto gH
\end{align*}

Let $R = \ker \phi$. Then $\phi: G \to K$ with $\ker \phi = R$.

Let $H = \ker \phi$. Then:
\begin{align*}
N(H) &= \{ g \in G \mid gHg^{-1} = H \} \\
&= \{ g \in G \mid gH = Hg \}
\end{align*}

Now:
\begin{align*}
g \in N(H) &\Leftrightarrow gH = Hg \\
&\Leftrightarrow gHg^{-1} = H \\
&\Leftrightarrow g \in N(H)
\end{align*}

Also:
\begin{align*}
g \in N(H) &\Leftrightarrow gH = Hg \\
&\Leftrightarrow (gH)(g^{-1}H) = H \\
&\Leftrightarrow gHg^{-1} = H
\end{align*}

Since $H \triangleleft G$, we have $N(H) = G$.

Now consider:
\begin{align*}
K &= G/H \\
k &\in K \Rightarrow k = gH \text{ for some } g \in G
\end{align*}

Then:
\begin{align*}
kH &= (gH)H = gH = k \\
Hk &= H(gH) = (Hg)H = (gH)H = gH = k
\end{align*}

So $H \triangleleft K$.

Now:
\begin{align*}
|K| &= |G/H| = [G:H] \\
|H| &= |\ker \phi|
\end{align*}

By the first isomorphism theorem:
\begin{align*}
G/\ker \phi &\cong \phi(G) \\
G/H &\cong K
\end{align*}

So $|G| = |H| \cdot |K|$.

Now let $K < G$ and $H < G$ with $H \triangleleft G$. Then:
\begin{align*}
KH &= \{ kh \mid k \in K, h \in H \} \\
HK &= \{ hk \mid h \in H, k \in K \}
\end{align*}

Since $H \triangleleft G$, we have $KH = HK$.

Also:
\begin{align*}
K \cap H &\triangleleft K \\
K/(K \cap H) &\cong KH/H
\end{align*}

By the second isomorphism theorem:
\begin{align*}
K/(K \cap H) &\cong KH/H
\end{align*}

Now if $K < N(H)$, then:
\begin{align*}
KH &= HK \\
|KH| &= \frac{|K||H|}{|K \cap H|}
\end{align*}

And:
\begin{align*}
[KH:H] &= [K:K \cap H]
\end{align*}

\end{document}